examples/bot/compile/README.md
@@ -1,11 +1,5 @@
 Compilation set up
 
-[arm7](arm7):
-arm6 compilation
-
-[arm8](arm8):
-arm8 compilation
-
 [botProgScript.sml](botProgScript.sml):
 Generic setup for compilation
 
